\documentclass{article}
\usepackage{amsmath}
\usepackage{tikz}
\usepackage{tikz-3dplot}
\usetikzlibrary{3d,angles,quotes,calc}
\newcommand{\fvec}[1]{\vec{\vphantom{A}#1}}
\begin{document}
\section{Linear algebra proofs}
\subsection{$ s(\fvec{a} + \fvec{b}) = s\fvec{a} + s\fvec{b} $}
$$ s(\fvec{a} + \fvec{b}) =
   s(\begin{bmatrix}a_1 \\ a_2 \\ ... \\ a_n\end{bmatrix} + \begin{bmatrix}b_1 \\ b_2 \\ ... \\ b_n\end{bmatrix}) =
   s\begin{bmatrix}a_1 + b_1 \\ a_2 + b_2 \\ ... \\ a_n + b_n\end{bmatrix} =
   \begin{bmatrix}s(a_1 + b_1) \\ s(a_2 + b_2) \\ ... \\ s(a_n + b_n)\end{bmatrix} $$
$$ = \begin{bmatrix}s a_1 + s b_1 \\ s a_2 + s b_2 \\ ... \\ s a_n + s b_n\end{bmatrix} =
   \begin{bmatrix}s a_1 \\ s a_2 \\ ... \\ s a_n\end{bmatrix} + \begin{bmatrix}s b_1 \\ s b_2 \\ ... \\ s b_n\end{bmatrix} =
   s\fvec{a} + s\fvec{b} $$

\subsection{$ \fvec{a} \times (\fvec{b} + \fvec{c}) = \fvec{a} \times \fvec{b} + \fvec{a} \times \fvec{c} $ if $ a, b, c \in R^{3} $}
$$ \fvec{a} \times (\fvec{b} + \fvec{c}) $$
$$ \begin{bmatrix} a_{x} \\ a_{y} \\ a_{z} \end{bmatrix} \times
    \left(\begin{bmatrix} b_{x} \\ b_{y} \\ b_{z} \end{bmatrix} + 
    \begin{bmatrix} c_{x} \\ c_{y} \\ c_{z} \end{bmatrix}\right) $$
$$ \begin{bmatrix} a_{x} \\ a_{y} \\ a_{z} \end{bmatrix} \times
    \begin{bmatrix} b_{x} + c_{x} \\ b_{y} + c_{y} \\ b_{z} + c_{z} \end{bmatrix} $$
$$ \begin{vmatrix}
    i & j & k \\
    a_{x} & a_{y} & a_{z} \\
    b_{x} + c_{x} & b_{y} + c_{y} & b_{z} + c_{z}
\end{vmatrix} $$
$$ a_{y}(b_{z} + c_{z})i + a_{z}(b_{x} + c_{x})j + a_{x}(b_{y} + c_{y})k - a_{y}(b_{x} + c_{x})k - a_{z}(b_{y} + c_{y})i - a_{x}(b_{z} + c_{z})j $$
$$ \begin{bmatrix}
    a_{y}(b_{z} + c_{z}) - a_{z}(b_{y} + c_{y}) \\
    a_{z}(b_{x} + c_{x}) - a_{x}(b_{z} + c_{z}) \\
    a_{x}(b_{y} + c_{y}) - a_{y}(b_{x} + c_{x})
\end{bmatrix} $$
$$ \begin{bmatrix}
    a_{y}b_{z} + a_{y}c_{z} - a_{z}b_{y} - a_{z}c_{y} \\
    a_{z}b_{x} + a_{z}c_{x} - a_{x}b_{z} - a_{x}c_{z} \\
    a_{x}b_{y} + a_{x}c_{y} - a_{y}b_{x} - a_{y}c_{x}
\end{bmatrix} $$
$$ \begin{bmatrix}
    (a_{y}b_{z} - a_{z}b_{y}) + (a_{y}c_{z} - a_{z}c_{y}) \\
    (a_{z}b_{x} - a_{x}b_{z}) + (a_{z}c_{x} - a_{x}c_{z}) \\
    (a_{x}b_{y} - a_{y}b_{x}) + (a_{x}c_{y} - a_{y}c_{x})
\end{bmatrix} $$
$$ \begin{bmatrix} a_{x} \\ a_{y} \\ a_{z} \end{bmatrix} \times
    \begin{bmatrix} b_{x} \\ b_{y} \\ b_{z} \end{bmatrix} + 
    \begin{bmatrix} a_{x} \\ a_{y} \\ a_{z} \end{bmatrix} \times
    \begin{bmatrix} c_{x} \\ c_{y} \\ c_{z} \end{bmatrix} $$
$$ \fvec{a} \times \fvec{b} + \fvec{a} \times \fvec{c} $$

\subsection{$ s(\fvec{a} \cdot \fvec{b}) = s\fvec{a} \cdot \fvec{b} = \fvec{a} \cdot s\fvec{b} $}
$$ \fvec{a} = \begin{bmatrix}a_1 \\ a_2 \\ ... \\ a_n\end{bmatrix}
    \fvec{b} = \begin{bmatrix}b_1 \\ b_2 \\ ... \\ b_n\end{bmatrix} $$

\noindent\begin{minipage}{.5\linewidth}
    $$ s(\fvec{a} \cdot \fvec{b}) $$
    $$ s(a_1 b_1 + a_2 b_2 + ... + a_n b_n) $$
    $$ s a_1 b_1 + s a_2 b_2 + ... + s a_n b_n $$
    $$ (s a_1) b_1 + (s a_2) b_2 + ... + (s a_n) b_n $$
    $$ s\fvec{a} \cdot \fvec{b} $$
\end{minipage}%
\hfill
\begin{minipage}{.5\linewidth}
    $$ s(\fvec{a} \cdot \fvec{b}) $$
    $$ s(a_1 b_1 + a_2 b_2 + ... + a_n b_n) $$
    $$ s a_1 b_1 + s a_2 b_2 + ... + s a_n b_n $$
    $$ a_1 s b_1 + a_2 s b_2 + ... + a_n s b_n $$
    $$ a_1 (s b_1) + a_2 (s b_2) + ... + a_n (s b_n) $$
    $$ \fvec{a} \cdot s\fvec{b} $$
\end{minipage}%

\subsection{$ |s| \cdot ||\fvec{a}|| = ||s\fvec{a}|| $}
$$ \fvec{a} \cdot \fvec{a} = ||\fvec{a}|| \cdot ||\fvec{a}|| cos(0) = ||\fvec{a}||^2 $$
$$ ||\fvec{a}|| = \sqrt{\fvec{a} \cdot \fvec{a}} $$

$$ ||s\fvec{a}|| $$
$$ \sqrt{s\fvec{a} \cdot s\fvec{a}} $$
$$ \sqrt{s(s\fvec{a} \cdot \fvec{a})} $$
$$ \sqrt{ss(\fvec{a} \cdot \fvec{a})} $$
$$ \sqrt{s^2}\sqrt{\fvec{a} \cdot \fvec{a}} $$
$$ |s|\sqrt{\fvec{a} \cdot \fvec{a}} $$
$$ |s| \cdot ||\fvec{a}|| $$

\subsection{$ s(\fvec{a} \times \fvec{b}) = s\fvec{a} \times \fvec{b} = \fvec{a} \times s\fvec{b} $}
\noindent\begin{minipage}{.5\linewidth}
    $$ s(\fvec{a} \times \fvec{b}) $$
    $$ s(||\fvec{a}|| \cdot ||\fvec{b}|| sin(\theta) \fvec{n}) $$
    If $ s \ge 0 $, 
    $$ ||s\fvec{a}|| \cdot ||\fvec{b}|| sin(\theta) \fvec{n} $$
    If $ s < 0 $, 
    $$ -||s\fvec{a}|| \cdot ||\fvec{b}|| sin(\theta + \frac{\pi}{2}) \fvec{n} $$
    $$ --||s\fvec{a}|| \cdot ||\fvec{b}|| sin(\theta) \fvec{n} $$
    $$ s\fvec{a} \times \fvec{b} $$
\end{minipage}%
\hfill
\begin{minipage}{.5\linewidth}
    $$ s(\fvec{a} \times \fvec{b}) $$
    $$ s(||\fvec{a}|| \cdot ||\fvec{b}|| sin(\theta) \fvec{n}) $$
    If $ s \ge 0 $, 
    $$ ||\fvec{a}|| \cdot ||s\fvec{b}|| sin(\theta) \fvec{n} $$
    If $ s < 0 $, 
    $$ -||\fvec{a}|| \cdot ||s\fvec{b}|| sin(\theta + \frac{\pi}{2}) \fvec{n} $$
    $$ --||\fvec{a}|| \cdot ||s\fvec{b}|| sin(\theta) \fvec{n} $$
    $$ \fvec{a} \times s\fvec{b} $$
\end{minipage}%

\subsection{Multiplying by a positive scalar does not affect a vector's orientation}
\noindent\begin{minipage}{.5\linewidth}
    $$ cos(\alpha) = \frac{\fvec{e_1} \cdot \fvec{a}}{||\fvec{a}||} $$
    \end{minipage}%
    \hfill
    \begin{minipage}{.5\linewidth}
    $$ \alpha = cos^{-1}\left(\frac{\fvec{e_1} \cdot \fvec{a}}{||\fvec{a}||}\right) $$
\end{minipage}%

$$ \alpha_{s\vec{a}} $$
$$ cos^{-1}\left(\frac{\fvec{e_1} \cdot s\fvec{a}}{||s\fvec{a}||}\right) $$
$$ cos^{-1}\left(\frac{s(\fvec{e_1} \cdot \fvec{a})}{|s| \cdot ||\fvec{a}||}\right) $$
Keep in mind that $ s \ge 0 $.
$$ cos^{-1}\left(\frac{\fvec{e_1} \cdot \fvec{a}}{||\fvec{a}||}\right) $$
$$ \alpha_{\vec{a}} $$

\section{Linear albgebra derivations}
\subsubsection{3D rotation formula}
\noindent\begin{minipage}{.5\linewidth}
    \tdplotsetmaincoords{30}{0} 
    \begin{tikzpicture} [scale=2, tdplot_main_coords, axis/.style={->,black,thick}, 
    vector/.style={-stealth,black,very thick}, 
    vector guide/.style={dashed,black,thick}]

    \coordinate (O) at (0,0,0);

    % vector to be rotated
    \pgfmathsetmacro{\vx}{0.8}
    \pgfmathsetmacro{\vy}{0}
    \pgfmathsetmacro{\vz}{0}
    \coordinate (V) at (\vx,\vy,\vz);

    % rotated vector
    \pgfmathsetmacro{\vx}{0.57}
    \pgfmathsetmacro{\vy}{0}
    \pgfmathsetmacro{\vz}{0.57}
    \coordinate (VP) at (\vx,\vy,\vz);

    % plane
    \draw[fill=gray,opacity=0.4] (-1,0,1) -- (1,0,1) -- (1,0,-1) -- (-1,0,-1) -- cycle;

    % draw rotation axis
    \draw[axis] (O) -- (0,1,0) node[anchor=south]{$ \vec{r} $};

    \draw[vector guide,->] (O) -- (0,0,-0.8) node[anchor=north]{$ \vec{r} \times \vec{v} $};

    % draw vectors
    \draw[vector] (O) -- (V) node[anchor=west]{$ \vec{v} $};
    \draw[vector] (O) -- (VP) node[anchor=west]{$ \vec{\,v}' $};

    % draw arc
    \pic [draw,angle radius=.6cm,angle eccentricity=1.4,"$\theta$"]
        {angle = V--O--VP};
    \end{tikzpicture}
\end{minipage}%
\hfill
\begin{minipage}{.5\linewidth}
    \tdplotsetmaincoords{90}{0} 
    \begin{tikzpicture} [scale=2, tdplot_main_coords, axis/.style={->,black,thick}, 
    vector/.style={-stealth,black,very thick}, 
    vector guide/.style={dashed,black,thick}]

    \coordinate (O) at (0,0,0);

    % vector to be rotated
    \pgfmathsetmacro{\vx}{0.8}
    \pgfmathsetmacro{\vy}{0}
    \pgfmathsetmacro{\vz}{0}
    \coordinate (V) at (\vx,\vy,\vz);

    % rotated vector
    \pgfmathsetmacro{\vpx}{0.57}
    \pgfmathsetmacro{\vpy}{0}
    \pgfmathsetmacro{\vpz}{0.57}
    \coordinate (VP) at (\vpx,\vpy,\vpz);

    % plane
    \draw[fill=gray,opacity=0.4] (-1,0,1) -- (1,0,1) -- (1,0,-1) -- (-1,0,-1) -- cycle;

    \draw[vector guide,->] (O) -- (0,0,-0.8) node[anchor=north]{$ \vec{r} \times \vec{v} $};

    % draw vectors
    \draw[vector] (O) -- (V) node[anchor=west]{$ \vec{v} $};
    \draw[vector] (O) -- (VP) node[anchor=west]{$ \vec{\,v}' $};

    % draw vector guides
    \draw[vector guide,->] (O) -- (0,0,\vpz) node[anchor=east]{$ sin(\theta)(\vec{r} \times \vec{v}) $};
        \draw[vector guide,->] (0,0,\vpz) -- (\vpx,0,\vpz) node[anchor=south]{$ cos(\theta)\vec{v} $};

    % draw arc
    \pic [draw,angle radius=.6cm,angle eccentricity=1.4,"$\theta$"]
        {angle = V--O--VP};
    \end{tikzpicture}
\end{minipage}%

If $ \fvec{v} \perp \fvec{r} $, $ \fvec{v^{\prime}} = cos(\theta) \fvec{v} + sin(\theta)(\fvec{r} \times \fvec{v}) $. We can therefore conclude that the general formula is $ \fvec{v^{\prime}} = cos(\theta) \fvec{v_{\perp}} + sin(\theta)(\fvec{r} \times \fvec{v_{\perp}}) + \fvec{v_{\parallel}} $. Let's substitute $ \fvec{v_{\perp}} $ for $ \fvec{v} - \fvec{v_{\parallel}} $

\noindent\begin{minipage}{.5\linewidth}
    \tdplotsetmaincoords{30}{0} 
    \begin{tikzpicture} [scale=2, tdplot_main_coords, axis/.style={->,black,thick}, 
    vector/.style={-stealth,black,very thick}, 
    vector guide/.style={dashed,black,thick}]

    \coordinate (O) at (0,0,0);

    % rotation vector
    \pgfmathsetmacro{\vx}{0.8}
    \pgfmathsetmacro{\vy}{0.8}
    \pgfmathsetmacro{\vz}{0.8}
    \coordinate (P) at (\vx,\vy,\vz);

    % plane
    \draw[fill=gray,opacity=0.4] (-1,0,1) -- (1,0,1) -- (1,0,-1) -- (-1,0,-1) -- cycle;

    % draw rotation axis
    \draw[axis] (0,0,0) -- (0,1,0) node[anchor=south]{$ \vec{r} $};

    % draw a vector from O to P
    \draw[vector] (O) -- (P) node[anchor=east]{$ \vec{v} $};

    % draw parallel and perpendicular vectors
    \draw[vector guide,->] (O) -- (\vx,0,\vz) node[anchor=west]{$ \vec{v}_{\perp} $};
    \draw[vector guide,->] (\vx,0,\vz) -- (P) node[anchor=west]{$ \vec{v}_{\parallel} $};
    \end{tikzpicture}
\end{minipage}%
\hfill
\begin{minipage}{.5\linewidth}
    $$ \fvec{v_{\parallel}} = proj_{\vec{r}} \fvec{v} = \frac{\fvec{v} \cdot \fvec{r}}{||\fvec{r}||} \cdot \fvec{r} $$
    Because $ ||\fvec{r}|| = 1 $, $ \fvec{v_{\parallel}} = (\fvec{v} \cdot \fvec{r}) \fvec{r} $.
\end{minipage}%

\begin{equation}
\begin{split}
\fvec{v^{\prime}} & = cos(\theta)(\fvec{v} - \fvec{v_{\parallel}}) + sin(\theta)(\fvec{r} \times (\fvec{v} - \fvec{v_{\parallel}})) + \fvec{v_{\parallel}} \\
& = cos(\theta) \fvec{v} - cos(\theta) \fvec{v_{\parallel}} + (\fvec{r} \times sin(\theta) (\fvec{v} - \fvec{v_{\parallel}})) + \fvec{v_{\parallel}} \\
& = cos(\theta) \fvec{v} - cos(\theta) \fvec{v_{\parallel}} + (\fvec{r} \times (sin(\theta) \fvec{v} - sin(\theta) \fvec{v_{\parallel}})) + \fvec{v_{\parallel}} \\
& = cos(\theta) \fvec{v} - cos(\theta) \fvec{v_{\parallel}} + (\fvec{r} \times sin(\theta) \fvec{v}) - (\fvec{r} \times sin(\theta) \fvec{v_{\parallel}}) + \fvec{v_{\parallel}} \\
& = cos(\theta) \fvec{v} - cos(\theta) \fvec{v_{\parallel}} + sin(\theta) (\fvec{r} \times \fvec{v}) - sin(\theta) (\fvec{r} \times \fvec{v_{\parallel}}) + \fvec{v_{\parallel}} \\
& = cos(\theta) \fvec{v} - cos(\theta) \fvec{v_{\parallel}} + sin(\theta) (\fvec{r} \times \fvec{v}) + \fvec{v_{\parallel}} \\
& = cos(\theta) \fvec{v} + (1 - cos(\theta))\fvec{v_{\parallel}} + sin(\theta) (\fvec{r} \times \fvec{v}) \\
& = cos(\theta) \fvec{v} + (1 - cos(\theta))(\fvec{v} \cdot \fvec{r}) \fvec{r} + sin(\theta) (\fvec{r} \times \fvec{v})
\end{split}
\end{equation}

\section{Quaternion derivations}
\subsubsection{Multiplication}
$$ i^2 = j^2 = k^2 = ijk = -1 $$
Substitution table:
\begin{tabular}{ |c|c|c|c| }
    \hline
      & i  & j  & k \\
    \hline
    i & -1 & k  & -j \\
    \hline
    j & -k & -1 & i \\
    \hline
    k & j  & -i & -1 \\
    \hline
\end{tabular}
\begin{equation}
\begin{split}
ab & = (a_{s} + a_{i}i + a_{j}j + a_{k}k)(b_{s} + b_{i}i + b_{j}j + b_{k}k) \\
    & = a_{s}b_{s} + a_{s}b_{i}i + a_{s}b_{j}j + a_{s}b_{k}k \\
    & \ \ \ + a_{i}ib_{s} + a_{i}ib_{i}i + a_{i}ib_{j}j + a_{i}ib_{k}k \\
    & \ \ \ + a_{j}jb_{s} + a_{j}jb_{i}i + a_{j}jb_{j}j + a_{j}jb_{k}k \\
    & \ \ \ + a_{k}kb_{s} + a_{k}kb_{i}i + a_{k}kb_{j}j + a_{k}kb_{k}k \\
    & = a_{s}b_{s} - a_{i}b_{i} - a_{j}b_{j} - a_{k}b_{k} \\
    & \ \ \ + a_{s}b_{i}i + a_{j}b_{k}i - a_{k}b_{j}i + a_{i}b_{s}i \\
    & \ \ \ + a_{s}b_{j}j + a_{k}b_{i}j - a_{i}b_{k}j + a_{j}b_{s}j \\
    & \ \ \ + a_{s}b_{k}k + a_{i}b_{j}k - a_{j}b_{i}k + a_{k}b_{s}k \\
    & = (a_{s}b_{s} - a_{i}b_{i} - a_{j}b_{j} - a_{k}b_{k}) \\
    & \ \ \ + (a_{i}b_{s} + a_{s}b_{i} - a_{k}b_{j} + a_{j}b_{k})i \\
    & \ \ \ + (a_{j}b_{s} + a_{k}b_{i} + a_{s}b_{j} - a_{i}b_{k})j \\
    & \ \ \ + (a_{k}b_{s} - a_{j}b_{i} + a_{i}b_{j} + a_{s}b_{k})k \\
    & = (a_{s}b_{s} - a_{i}b_{i} - a_{j}b_{j} - a_{k}b_{k} \\
    & \ \ \ \ , a_{i}b_{s} + a_{s}b_{i} - a_{k}b_{j} + a_{j}b_{k} \\
    & \ \ \ \ , a_{j}b_{s} + a_{k}b_{i} + a_{s}b_{j} - a_{i}b_{k} \\
    & \ \ \ \ , a_{k}b_{s} - a_{j}b_{i} + a_{i}b_{j} + a_{s}b_{k})
\end{split}
\end{equation}

\subsubsection{Multiplication in matrix form}
$$ \begin{bmatrix}
    a_{s} & -a_{i} & -a_{j} & -a_{k} \\
    a_{i} & a_{s} & -a_{k} & a_{j} \\
    a_{j} & a_{k} & a_{s} & -a_{i} \\
    a_{k} & -a_{j} & a_{i} & a_{s}
\end{bmatrix}
\begin{bmatrix} b_{s} \\ b_{i} \\ b_{j} \\ b_{k} \end{bmatrix} =
\begin{bmatrix}
    (a_{s}b_{s} - a_{i}b_{i} - a_{j}b_{j} - a_{k}b_{k} \\
    a_{i}b_{s} + a_{s}b_{i} - a_{k}b_{j} + a_{j}b_{k} \\
    a_{j}b_{s} + a_{k}b_{i} + a_{s}b_{j} - a_{i}b_{k} \\
    a_{k}b_{s} - a_{j}b_{i} + a_{i}b_{j} + a_{s}b_{k}
\end{bmatrix} $$

\subsubsection{Multiplication in vector form}
\begin{equation}
\begin{split}
ab & = (a_{s} + a_{i}i + a_{j}j + a_{k}k)(b_{s} + b_{i}i + b_{j}j + b_{k}k) \\
    & = (a_{s}b_{s} - a_{i}b_{i} - a_{j}b_{j} - a_{k}b_{k} \\
    & \ \ \ \ , a_{i}b_{s} + a_{s}b_{i} - a_{k}b_{j} + a_{j}b_{k} \\
    & \ \ \ \ , a_{j}b_{s} + a_{k}b_{i} + a_{s}b_{j} - a_{i}b_{k} \\
    & \ \ \ \ , a_{k}b_{s} - a_{j}b_{i} + a_{i}b_{j} + a_{s}b_{k}) \\
    & = (a_{s}b_{s} - (a_{i}b_{i} + a_{j}b_{j} + a_{k}b_{k}) \\
    & \ \ \ \ , a_{s}b_{i} + a_{j}b_{k} - a_{k}b_{j} + a_{i}b_{s} \\
    & \ \ \ \ , a_{s}b_{j} + a_{k}b_{i} - a_{i}b_{k} + a_{j}b_{s} \\
    & \ \ \ \ , a_{s}b_{k} + a_{i}b_{j} - a_{j}b_{i} + a_{k}b_{s}) \\
    & = (a_{s}, \fvec{a}_{v})(b_{s}, \fvec{b}_{v}) \\
    & = (a_{s} b_{s} - \fvec{a}_{v} \cdot \fvec{b}_{v}, \, a_{s} \fvec{b}_{v} + b_{s} \fvec{a}_{v} + \fvec{a}_{v} \times \fvec{b}_{v}) \\
\end{split}
\end{equation}

\subsubsection{Cross product in quaternionic form}
$$ xy = (0, \fvec{x})(0, \fvec{y}) = (-\fvec{x} \cdot \fvec{y}, \fvec{x} \times \fvec{y}) $$
$$ yx = (0, \fvec{y})(0, \fvec{x}) = (-\fvec{y} \cdot \fvec{x}, \fvec{y} \times \fvec{x}) = (-\fvec{x} \cdot \fvec{y}, -\fvec{x} \times \fvec{y}) $$
$$ xy - yx = (-\fvec{x} \cdot \fvec{y}, \fvec{x} \times \fvec{y}) - (-\fvec{x} \cdot \fvec{y}, -\fvec{x} \times \fvec{y}) = (0, 2(\fvec{x} \times \fvec{y})) $$
$$ \fvec{x} \times \fvec{y} = \frac{1}{2}(xy - yx) $$

\subsubsection{3D rotation formula}
\noindent\begin{minipage}{.4\linewidth}
    $$ v = (0, \vec{v}) $$
    $$ v_{\perp} = (0, \vec{v}_{\perp}) $$
    $$ v_{\parallel} = (0, \vec{v}_{\parallel}) $$
    $$ v' = (0, \vec{v}\,') $$
    $$ r = (0, \vec{r}) $$
    $$ rv = (\vec{r} \cdot \vec{v}, \vec{r} \times \vec{v}) $$
    $$ (a, 0)(b, \vec{x}) = (ab, a\vec{x}) $$
\end{minipage}%
\hfill
\begin{minipage}{.6\linewidth}
    If $ \fvec{v} \perp \fvec{r} $, $ \fvec{v^{\prime}} = cos(\theta) \fvec{v} + sin(\theta)(\fvec{r} \times \fvec{v}) $.
    \begin{equation}
    \begin{split}
        v' & = cos(\theta)v + sin(\theta)rv \\
           & = (cos(\theta) + sin(\theta)r)v \\
           & = e^{\theta r}v \\
           & = (cos(\theta), sin(\theta)\fvec{r})(0, \fvec{v}) \\
           & = (-sin(\theta)\fvec{r} \cdot \fvec{v}, cos(\theta) \fvec{v} + sin(\theta)\fvec{r} \times \fvec{v}) \\
           & = (-\fvec{v} \cdot sin(\theta)\fvec{r}, cos(\theta) \fvec{v} - \fvec{v} \times sin(\theta)\fvec{r}) \\
           & = (0, \fvec{v})(cos(\theta), -sin(\theta)\fvec{r}) \\
           & = ve^{-\theta r} \\
    \end{split}
    \end{equation}
\end{minipage}%

If $ \fvec{v} $ not $ \perp \fvec{r} $,
\begin{equation}
\begin{split}
    v' & = v_{\parallel} + v_{\perp}e^{-\theta r} \\
       & = e^{\frac{\theta}{2}r}e^{-\frac{\theta}{2} r}(v_{\parallel} + v_{\perp}e^{-\theta r}) \\
       & = e^{\frac{\theta}{2}r}e^{-\frac{\theta}{2} r}v_{\parallel} + e^{\frac{\theta}{2}r}e^{-\frac{\theta}{2} r}v_{\perp}e^{-\theta r} \\
       & = e^{\frac{\theta}{2}r}e^{-\frac{\theta}{2} r}v_{\parallel} + e^{\frac{\theta}{2}r}e^{\frac{\theta}{2} r}v_{\perp} \\
       & = e^{\frac{\theta}{2}r}e^{-\frac{\theta}{2} r}v_{\parallel} + e^{\frac{\theta}{2}r}v_{\perp}e^{-\frac{\theta}{2} r} \\
       & = e^{\frac{\theta}{2}r}(cos(-\frac{\theta}{2}), sin(-\frac{\theta}{2})\fvec{r})(0,\fvec{v}_{\parallel}) + e^{\frac{\theta}{2}r}v_{\perp}e^{-\frac{\theta}{2} r} \\
       & = e^{\frac{\theta}{2}r}(-(cos(-\frac{\theta}{2})\fvec{r}) \cdot \fvec{v}_{\parallel},cos(-\frac{\theta}{2})\fvec{v}_{\parallel} + (sin(-\frac{\theta}{2})\fvec{r}) \times \fvec{v}_{\parallel}) + e^{\frac{\theta}{2}r}v_{\perp}e^{-\frac{\theta}{2} r} \\
       & = e^{\frac{\theta}{2}r}(-\fvec{v}_{\parallel} \cdot (cos(-\frac{\theta}{2})\fvec{r}), cos(-\frac{\theta}{2})\fvec{v}_{\parallel} - \fvec{v}_{\parallel} \times (sin(-\frac{\theta}{2})\fvec{r})) + e^{\frac{\theta}{2}r}v_{\perp}e^{-\frac{\theta}{2} r} \\
       & = e^{\frac{\theta}{2}r}(0,\fvec{v}_{\parallel})(cos(-\frac{\theta}{2}), sin(-\frac{\theta}{2})\fvec{r}) + e^{-\frac{\theta}{2}r}v_{\perp}e^{-\frac{\theta}{2} r} \\
       & = e^{\frac{\theta}{2}r}v_{\parallel}e^{-\frac{\theta}{2} r} + e^{\frac{\theta}{2}r}v_{\perp}e^{-\frac{\theta}{2} r} \\
       & = e^{\frac{\theta}{2}r}(v_{\parallel} + v_{\perp})e^{-\frac{\theta}{2} r} \\
       & = e^{\frac{\theta}{2}r}ve^{-\frac{\theta}{2} r} \\
\end{split}
\end{equation}
\end{document}
